pulse/share/steel/examples/pulse/Fibonacci.fst
@@ -11,143 +11,141 @@ let rec fib_mono (n:nat) (m:nat { m <= n})
     (ensures fib m <= fib n)
   = if n = m then ()
     else fib_mono (n - 1) m
-
-#push-options "--using_facts_from 'Prims FStar.Pervasives FStar.Ghost FStar.UInt FStar.UInt32 Fibonacci'"
+open FStar.UInt32
+open Pulse.Class.BoundedIntegers
+#push-options "--using_facts_from '* -FStar.Tactics -FStar.Reflection'"
 
 ```pulse
-fn fibo32 (k:(n:U32.t { 0 < U32.v n  /\ fib (U32.v n) < pow2 32 }))
-  requires emp
+fn fibo32 (k:U32.t)
+  requires pure (0ul < k /\ fib (v k) < pow2 32)
   returns r:U32.t
-  ensures pure (U32.v r == fib (U32.v k))
+  ensures pure (v r == fib (v k))
 {
   let mut i = 1ul;
   let mut j = 1ul;
   let mut ctr = 1ul;
-  while (let vctr = !ctr; U32.(vctr <^ k))
-  invariant b . exists vi vj vctr. (
-     pts_to i vi `star`
-     pts_to j vj `star`
-     pts_to ctr vctr `star`     
-     pure (1 <= U32.v vctr /\
-           U32.v vctr <= U32.v k /\
-           fib (U32.v vctr - 1) == U32.v vi/\
-           fib (U32.v vctr) == U32.v vj /\
-           b == U32.(vctr <^ k))
-  )
+  while ((ctr < k))
+  invariant b . 
+    exists vi vj vctr. 
+     pts_to i vi **
+     pts_to j vj **
+     pts_to ctr vctr **
+     pure (1ul <=  vctr /\
+           vctr <= k /\
+           fib (v vctr - 1) == v vi/\
+           fib (v vctr) == v vj /\
+           b == (vctr < k))
   {
-     let vc = !ctr;
-     let vi = !i;
-     let vj = !j;
-     ctr := U32.(vc +^ 1ul);
-     i := vj;
-     fib_mono (U32.v k) (U32.v vc + 1);
-     j := U32.(vi +^ vj);
-     ()
+     let vi = i;
+     ctr := ctr + 1ul;
+     fib_mono (v k) (v ctr);
+     i := j;
+     j := vi + j;
   };
-  let r = !j;
-  r
+  j
 }
 ```
 
 
-```pulse
-fn fibo (n:pos)
-  requires emp
-  returns r:int
-  ensures pure (r == fib n)
-{
-  let mut i = 1;
-  let mut j = 1;
-  let mut ctr = 1;
-  while (let vctr = !ctr; (vctr < n))
-  invariant b . exists vi vj vctr. (
-     pts_to i vi `star`
-     pts_to j vj `star`
-     pts_to ctr vctr `star`     
-     pure (1 <= vctr /\
-           vctr <= n /\
-           vi == fib (vctr - 1) /\
-           vj == fib vctr /\
-           b == (vctr < n))
-  )
-  {
-     let vc = !ctr;
-     let vi = !i;
-     let vj = !j;
-     i := vj;
-     j := vi + vj;
-     ctr := vc + 1;
-     ()
-  };
-  let r = !j;
-  r
-}
-```
+// ```pulse
+// fn fibo (n:pos)
+//   requires emp
+//   returns r:int
+//   ensures pure (r == fib n)
+// {
+//   let mut i = 1;
+//   let mut j = 1;
+//   let mut ctr = 1;
+//   while (let vctr = !ctr; (vctr < n))
+//   invariant b . exists vi vj vctr. (
+//      pts_to i vi `star`
+//      pts_to j vj `star`
+//      pts_to ctr vctr `star`     
+//      pure (1 <= vctr /\
+//            vctr <= n /\
+//            vi == fib (vctr - 1) /\
+//            vj == fib vctr /\
+//            b == (vctr < n))
+//   )
+//   {
+//      let vc = !ctr;
+//      let vi = !i;
+//      let vj = !j;
+//      i := vj;
+//      j := vi + vj;
+//      ctr := vc + 1;
+//      ()
+//   };
+//   let r = !j;
+//   r
+// }
+// ```
 
-```pulse
-fn fibo2 (n:pos)
-  requires emp
-  returns r:nat
-  ensures pure (r == fib n)
-{
-  let mut i = ( 1 <: nat );
-  let mut j = ( 1 <: nat );
-  let mut ctr = ( 1 <: pos );
-  while (let vctr = !ctr; (vctr < n))
-  invariant b . exists vi vj vctr. (
-     pts_to i vi `star`
-     pts_to j vj `star`
-     pts_to ctr vctr `star`     
-     pure (1 <= vctr /\
-           vctr <= n /\
-           vi == fib (vctr - 1) /\
-           vj == fib vctr /\
-           b == (vctr < n))
-  )
-  {
-     let vc = !ctr;
-     let vi = !i;
-     let vj = !j;
-     i := vj;
-     j := vi + vj;
-     ctr := vc + 1;
-     ()
-  };
-  let r = !j;
-  r
-}
-```
+// ```pulse
+// fn fibo2 (n:pos)
+//   requires emp
+//   returns r:nat
+//   ensures pure (r == fib n)
+// {
+//   let mut i = ( 1 <: nat );
+//   let mut j = ( 1 <: nat );
+//   let mut ctr = ( 1 <: pos );
+//   while (let vctr = !ctr; (vctr < n))
+//   invariant b . exists vi vj vctr. (
+//      pts_to i vi `star`
+//      pts_to j vj `star`
+//      pts_to ctr vctr `star`     
+//      pure (1 <= vctr /\
+//            vctr <= n /\
+//            vi == fib (vctr - 1) /\
+//            vj == fib vctr /\
+//            b == (vctr < n))
+//   )
+//   {
+//      let vc = !ctr;
+//      let vi = !i;
+//      let vj = !j;
+//      i := vj;
+//      j := vi + vj;
+//      ctr := vc + 1;
+//      ()
+//   };
+//   let r = !j;
+//   r
+// }
+// ```
 
-```pulse
-fn fibo3 (n:pos)
-  requires emp
-  returns r: (r:nat { r == fib n })
-  ensures emp
-{
-  let mut i = ( 1 <: nat );
-  let mut j = ( 1 <: nat );
-  let mut ctr = ( 1 <: pos );
-  while (let vctr = !ctr; (vctr < n))
-  invariant b . exists vi vj vctr. (
-     pts_to i vi `star`
-     pts_to j vj `star`
-     pts_to ctr vctr `star`     
-     pure (1 <= vctr /\
-           vctr <= n /\
-           vi == fib (vctr - 1) /\
-           vj == fib vctr /\
-           b == (vctr < n))
-  )
-  {
-     let vc = !ctr;
-     let vi = !i;
-     let vj = !j;
-     i := vj;
-     j := vi + vj;
-     ctr := vc + 1;
-     ()
-  };
-  let r = !j;
-  r
-}
-```
+// ```pulse
+// fn fibo3 (n:pos)
+//   requires emp
+//   returns r: (r:nat { r == fib n })
+//   ensures emp
+// {
+//   let mut i = ( 1 <: nat );
+//   let mut j = ( 1 <: nat );
+//   let mut ctr = ( 1 <: pos );
+//   while (let vctr = !ctr; (vctr < n))
+//   invariant b . exists vi vj vctr. (
+//      pts_to i vi `star`
+//      pts_to j vj `star`
+//      pts_to ctr vctr `star`     
+//      pure (1 <= vctr /\
+//            vctr <= n /\
+//            vi == fib (vctr - 1) /\
+//            vj == fib vctr /\
+//            b == (vctr < n))
+//   )
+//   {
+//      let vc = !ctr;
+//      let vi = !i;
+//      let vj = !j;
+//      i := vj;
+//      j := vi + vj;
+//      ctr := vc + 1;
+//      ()
+//   };
+//   let r = !j;
+//   r
+// }
+// ```
+ 
