pulse/src/syntax_extension/Pulse_ASTBuilder.fst
@@ -81,6 +81,6 @@ let parse_pulse (env:TcEnv.env)
       R.mk_range file_name p p
     in
     match Pulse.Parser.parse_decl content range with
-    | Inl d -> D.desugar_decl env d
+    | Inl d -> fst (D.desugar_decl env d 0)
     | Inr e -> Inr e
     
